README.md
@@ -3,3 +3,10 @@
 Run ```coq_makefile -f _CoqProject -o CoqMakefile``` to update Makefile.  
 Run ```rm .*.aux && make clean ``` to clean the compiled files.  
 Run ```make``` to compile the files.  
+
+To use simplify quantum expressions, you can use the script ```MatricesConverter.py``` as follows:
+```
+python3 MatricesConverter.py
+enter expression: [ENTER EXPRESSION]
+enter name: [ENTER NAME]
+```
